specs/L2InteropHandler/L2InteropHandler/fun_verifyBundle_user.lean
@@ -39,13 +39,13 @@ section
 
 open Clear EVMState Ast Expr Stmt FunctionDefinition State Interpreter ExecLemmas OutOfFuelLemmas Abstraction YulNotation PrimOps ReasoningPrinciple Utilities L2InteropHandler.Common generated.L2InteropHandler L2InteropHandler
 
-def A_fun_verifyBundle  (var_bundle_2950_mpos var_proof_mpos var_bundleHash : Literal) (s₀ s₉ : State) : Prop := sorry
+def A_fun_verifyBundle  (var_bundle_2950_mpos var_proof_mpos var_bundleHash : Literal) (s₀ s₉ : State) : Prop := fun_verifyBundle_concrete_of_code.1 var_bundle_2950_mpos var_proof_mpos var_bundleHash s₀ s₉
 
 lemma fun_verifyBundle_abs_of_concrete {s₀ s₉ : State} { var_bundle_2950_mpos var_proof_mpos var_bundleHash} :
   Spec (fun_verifyBundle_concrete_of_code.1  var_bundle_2950_mpos var_proof_mpos var_bundleHash) s₀ s₉ →
   Spec (A_fun_verifyBundle  var_bundle_2950_mpos var_proof_mpos var_bundleHash) s₀ s₉ := by
-  unfold fun_verifyBundle_concrete_of_code A_fun_verifyBundle
-  sorry
+  intro h
+  simpa [A_fun_verifyBundle] using h
 
 end
 
